lifter: sort out distinct labels properly
Before, we checked that the address labels were distinct by demanding
that their numeric values are strictly sorted and just used brute force
on the string labels. Since for our current examples, there are no
string labels, this worked fine.

Now, we demand formally that the string labels are prefixed with a
string version of their corresponding address label. This was an
informal requirement before anyhow. By making it formal, we can show
that we don't need to consider the string labels at all. Moreover, the
sorting trick for the address labels has been cleaned up.

src/tools/lifter/bir_inst_liftingLib.sml
@@ -7,6 +7,7 @@ open bir_exp_liftingLib bir_typing_expSyntax
 open bir_typing_expTheory
 open bir_lifter_general_auxTheory
 open bir_programSyntax bir_interval_expSyntax
+open bir_program_labelsTheory
 open PPBackEnd Parse
 
 (**********)
@@ -1421,19 +1422,8 @@ functor bir_inst_liftingFunctor (MD : sig val mr : bmr_rec end) : bir_inst_lifti
       val prog_thm = let
         val thm0 = MATCH_MP prog_dist_ELIM_THM prog_dist_thm_clean
         val (pre, _) = dest_imp_only (concl thm0)
-
-        val pre_thm0 = SPEC (rand pre) ALL_DISTINCT_lifter_label_list_PARTS_THM
-
-        val pre0 = lhs (fst (dest_imp_only (snd (strip_forall (concl pre_thm0)))))
-        val pre0_thm = (PURE_REWRITE_CONV (combinTheory.K_THM::bir_labels_of_program_EVAL::ALL_DISTINCT_lifter_labels_list_PART_def::bir_block_rewrs) THENC EVAL) pre0
-
-        val pre_thm1 = MATCH_MP pre_thm0 pre0_thm
-
-        val pre1 = (fst (dest_imp_only (concl pre_thm1)))
-        val pre1_thm = EQT_ELIM (EVAL pre1)
-        val pre_thm2 = MATCH_MP pre_thm1 pre1_thm
-
-        val thm1 = MP thm0 pre_thm2
+        val pre_thm = EQT_ELIM (EVAL pre)
+        val thm1 = MP thm0 pre_thm
       in thm1 end
     in
       (prog_thm, List.rev (!failing_inst_r))
